src/fs/Interpreter.fs
@@ -22,7 +22,7 @@ end
 | ExprTypes.ARRAY (lst) -> begin
 (isVal_lst lst)
 end
-| _18_20 -> begin
+| _21_20 -> begin
 false
 end))
 and isVal_lst : ExprTypes.l__GExpr Prims.list  ->  Prims.bool = (fun ( lst  :  ExprTypes.l__GExpr Prims.list ) -> (match (lst) with
@@ -32,7 +32,7 @@ end
 | ExprTypes.LOC (l)::xs -> begin
 (isVal_lst xs)
 end
-| _18_28 -> begin
+| _21_28 -> begin
 false
 end))
 
@@ -47,7 +47,7 @@ end
 | ExprTypes.BOOL (b) -> begin
 true
 end
-| _18_37 -> begin
+| _21_37 -> begin
 false
 end))
 
@@ -80,14 +80,14 @@ end
 end))
 
 
-let rec step = (fun ( _18_57  :  'Astate config ) ( interp  :  'Astate interpretation ) -> (match (_18_57) with
+let rec step = (fun ( _21_57  :  'Astate config ) ( interp  :  'Astate interpretation ) -> (match (_21_57) with
 | (tm, st) -> begin
 (match (tm) with
 | ExprTypes.LET (x, t1, t2) -> begin
 if (isVal t1) then begin
 Util.Val (((ExprTypes.substGExpr t2 x t1), st))
 end else begin
-(Util.bindT (step (t1, st) interp) (fun ( _18_66  :  'Astate config ) -> (match (_18_66) with
+(Util.bindT (step (t1, st) interp) (fun ( _21_66  :  'Astate config ) -> (match (_21_66) with
 | (t1', st') -> begin
 Util.Val ((ExprTypes.LET ((x, t1', t2)), st'))
 end)))
@@ -95,13 +95,13 @@ end
 end
 | ExprTypes.APPLY (t1, t2) -> begin
 if (not ((isVal t1))) then begin
-(Util.bindT (step (t1, st) interp) (fun ( _18_73  :  'Astate config ) -> (match (_18_73) with
+(Util.bindT (step (t1, st) interp) (fun ( _21_73  :  'Astate config ) -> (match (_21_73) with
 | (t1', st') -> begin
 Util.Val ((ExprTypes.APPLY ((t1', t2)), st'))
 end)))
 end else begin
 if (not ((isVal t2))) then begin
-(Util.bindT (step (t2, st) interp) (fun ( _18_76  :  'Astate config ) -> (match (_18_76) with
+(Util.bindT (step (t2, st) interp) (fun ( _21_76  :  'Astate config ) -> (match (_21_76) with
 | (t2', st') -> begin
 Util.Val ((ExprTypes.APPLY ((t1, t2')), st'))
 end)))
@@ -110,7 +110,7 @@ end else begin
 | ExprTypes.LAMBDA (x, ty, t) -> begin
 Util.Val (((ExprTypes.substGExpr t x t2), st))
 end
-| _18_83 -> begin
+| _21_83 -> begin
 Util.Err ((FStar.String.strcat "Cannot reduce application: " (ExprTypes.show tm)))
 end)
 end
@@ -118,7 +118,7 @@ end
 end
 | ExprTypes.SEQUENCE (t1, t2) -> begin
 if (not ((isVal t1))) then begin
-(Util.bindT (step (t1, st) interp) (fun ( _18_90  :  'Astate config ) -> (match (_18_90) with
+(Util.bindT (step (t1, st) interp) (fun ( _21_90  :  'Astate config ) -> (match (_21_90) with
 | (t1', st') -> begin
 Util.Val ((ExprTypes.SEQUENCE ((t1', t2)), st'))
 end)))
@@ -127,20 +127,20 @@ end else begin
 | ExprTypes.UNIT -> begin
 Util.Val ((t2, st))
 end
-| _18_93 -> begin
+| _21_93 -> begin
 Util.Err ((FStar.String.strcat "Cannot reduce sequence: " (ExprTypes.show tm)))
 end)
 end
 end
 | ExprTypes.ASSIGN (t1, t2) -> begin
 if (not ((isVal t1))) then begin
-(Util.bindT (step (t1, st) interp) (fun ( _18_100  :  'Astate config ) -> (match (_18_100) with
+(Util.bindT (step (t1, st) interp) (fun ( _21_100  :  'Astate config ) -> (match (_21_100) with
 | (t1', st') -> begin
 Util.Val ((ExprTypes.ASSIGN ((t1', t2)), st'))
 end)))
 end else begin
 if (not ((isBexp t2))) then begin
-(Util.bindT (step (t2, st) interp) (fun ( _18_103  :  'Astate config ) -> (match (_18_103) with
+(Util.bindT (step (t2, st) interp) (fun ( _21_103  :  'Astate config ) -> (match (_21_103) with
 | (t2', st') -> begin
 Util.Val ((ExprTypes.ASSIGN ((t1, t2')), st'))
 end)))
@@ -149,7 +149,7 @@ end else begin
 | ExprTypes.LOC (l) -> begin
 Util.Val ((ExprTypes.UNIT, (interp.assign st l (get_bexp t2))))
 end
-| _18_107 -> begin
+| _21_107 -> begin
 Util.Err ((FStar.String.strcat "Cannot reduce assignment: " (ExprTypes.show tm)))
 end)
 end
@@ -157,13 +157,13 @@ end
 end
 | ExprTypes.XOR (t1, t2) -> begin
 if (not ((isBexp t1))) then begin
-(Util.bindT (step (t1, st) interp) (fun ( _18_114  :  'Astate config ) -> (match (_18_114) with
+(Util.bindT (step (t1, st) interp) (fun ( _21_114  :  'Astate config ) -> (match (_21_114) with
 | (t1', st') -> begin
 Util.Val ((ExprTypes.XOR ((t1', t2)), st'))
 end)))
 end else begin
 if (not ((isBexp t2))) then begin
-(Util.bindT (step (t2, st) interp) (fun ( _18_117  :  'Astate config ) -> (match (_18_117) with
+(Util.bindT (step (t2, st) interp) (fun ( _21_117  :  'Astate config ) -> (match (_21_117) with
 | (t2', st') -> begin
 Util.Val ((ExprTypes.XOR ((t1, t2')), st'))
 end)))
@@ -174,13 +174,13 @@ end
 end
 | ExprTypes.AND (t1, t2) -> begin
 if (not ((isBexp t1))) then begin
-(Util.bindT (step (t1, st) interp) (fun ( _18_124  :  'Astate config ) -> (match (_18_124) with
+(Util.bindT (step (t1, st) interp) (fun ( _21_124  :  'Astate config ) -> (match (_21_124) with
 | (t1', st') -> begin
 Util.Val ((ExprTypes.AND ((t1', t2)), st'))
 end)))
 end else begin
 if (not ((isBexp t2))) then begin
-(Util.bindT (step (t2, st) interp) (fun ( _18_127  :  'Astate config ) -> (match (_18_127) with
+(Util.bindT (step (t2, st) interp) (fun ( _21_127  :  'Astate config ) -> (match (_21_127) with
 | (t2', st') -> begin
 Util.Val ((ExprTypes.AND ((t1, t2')), st'))
 end)))
@@ -201,13 +201,13 @@ in Util.Val ((ExprTypes.BEXP (bexp), st)))
 end
 | ExprTypes.APPEND (t1, t2) -> begin
 if (not ((isVal t1))) then begin
-(Util.bindT (step (t1, st) interp) (fun ( _18_137  :  'Astate config ) -> (match (_18_137) with
+(Util.bindT (step (t1, st) interp) (fun ( _21_137  :  'Astate config ) -> (match (_21_137) with
 | (t1', st') -> begin
 Util.Val ((ExprTypes.APPLY ((t1', t2)), st'))
 end)))
 end else begin
 if (not ((isVal t2))) then begin
-(Util.bindT (step (t2, st) interp) (fun ( _18_140  :  'Astate config ) -> (match (_18_140) with
+(Util.bindT (step (t2, st) interp) (fun ( _21_140  :  'Astate config ) -> (match (_21_140) with
 | (t2', st') -> begin
 Util.Val ((ExprTypes.APPLY ((t1, t2')), st'))
 end)))
@@ -216,7 +216,7 @@ end else begin
 | (ExprTypes.ARRAY (l), ExprTypes.ARRAY (l')) -> begin
 Util.Val ((ExprTypes.ARRAY ((FStar.List.append l l')), st))
 end
-| _18_147 -> begin
+| _21_147 -> begin
 Util.Err ((FStar.String.strcat "Cannot reduce append: " (ExprTypes.show tm)))
 end)
 end
@@ -224,73 +224,73 @@ end
 end
 | ExprTypes.ROT (i, t) -> begin
 if (not ((isVal t))) then begin
-(Util.bindT (step (t, st) interp) (fun ( _18_154  :  'Astate config ) -> (match (_18_154) with
+(Util.bindT (step (t, st) interp) (fun ( _21_154  :  'Astate config ) -> (match (_21_154) with
 | (t', st') -> begin
 Util.Val ((ExprTypes.ROT ((i, t')), st'))
 end)))
 end else begin
 (match (t) with
 | ExprTypes.ARRAY (lst) -> begin
-if ((0 <= i) && (i < (FStar.List.lengthT lst))) then begin
+if (((Prims.parse_int "0") <= i) && (i < (FStar.List.lengthT lst))) then begin
 Util.Val ((ExprTypes.ARRAY ((Util.rotate lst i)), st))
 end else begin
 Util.Err ((FStar.String.strcat "Array out of bounds: " (ExprTypes.show tm)))
 end
 end
-| _18_158 -> begin
+| _21_158 -> begin
 Util.Err ((FStar.String.strcat "Cannot reduce rotation: " (ExprTypes.show tm)))
 end)
 end
 end
 | ExprTypes.SLICE (t, i, j) -> begin
 if (not ((isVal t))) then begin
-(Util.bindT (step (t, st) interp) (fun ( _18_166  :  'Astate config ) -> (match (_18_166) with
+(Util.bindT (step (t, st) interp) (fun ( _21_166  :  'Astate config ) -> (match (_21_166) with
 | (t', st') -> begin
 Util.Val ((ExprTypes.SLICE ((t', i, j)), st'))
 end)))
 end else begin
 (match (t) with
 | ExprTypes.ARRAY (lst) -> begin
-if (((0 <= i) && (i <= j)) && (j < (FStar.List.lengthT lst))) then begin
+if ((((Prims.parse_int "0") <= i) && (i <= j)) && (j < (FStar.List.lengthT lst))) then begin
 Util.Val ((ExprTypes.ARRAY ((Util.slice lst i j)), st))
 end else begin
 Util.Err ((FStar.String.strcat "Array out of bounds: " (ExprTypes.show tm)))
 end
 end
-| _18_170 -> begin
+| _21_170 -> begin
 Util.Err ((FStar.String.strcat "Cannot reduce slice: " (ExprTypes.show tm)))
 end)
 end
 end
 | ExprTypes.ARRAY (lst) -> begin
-(Util.bindT (step_lst (lst, st) interp) (fun ( _18_175  :  'Astate listconfig ) -> (match (_18_175) with
+(Util.bindT (step_lst (lst, st) interp) (fun ( _21_175  :  'Astate listconfig ) -> (match (_21_175) with
 | (lst, st') -> begin
 Util.Val ((ExprTypes.ARRAY (lst), st'))
 end)))
 end
 | ExprTypes.GET_ARRAY (t, i) -> begin
 if (not ((isVal t))) then begin
-(Util.bindT (step (t, st) interp) (fun ( _18_182  :  'Astate config ) -> (match (_18_182) with
+(Util.bindT (step (t, st) interp) (fun ( _21_182  :  'Astate config ) -> (match (_21_182) with
 | (t', st') -> begin
 Util.Val ((ExprTypes.GET_ARRAY ((t', i)), st'))
 end)))
 end else begin
 (match (t) with
 | ExprTypes.ARRAY (lst) -> begin
-if ((0 <= i) && (i < (FStar.List.lengthT lst))) then begin
+if (((Prims.parse_int "0") <= i) && (i < (FStar.List.lengthT lst))) then begin
 Util.Val (((Util.nthT lst i), st))
 end else begin
 Util.Err ((FStar.String.strcat "Array out of bounds: " (ExprTypes.show tm)))
 end
 end
-| _18_186 -> begin
+| _21_186 -> begin
 Util.Err ((FStar.String.strcat "Cannot reduce array index: " (ExprTypes.show tm)))
 end)
 end
 end
 | ExprTypes.ASSERT (t) -> begin
 if (not ((isVal t))) then begin
-(Util.bindT (step (t, st) interp) (fun ( _18_191  :  'Astate config ) -> (match (_18_191) with
+(Util.bindT (step (t, st) interp) (fun ( _21_191  :  'Astate config ) -> (match (_21_191) with
 | (t', st') -> begin
 Util.Val ((ExprTypes.ASSERT (t'), st'))
 end)))
@@ -299,7 +299,7 @@ end else begin
 | ExprTypes.LOC (l) -> begin
 Util.Val ((ExprTypes.UNIT, st))
 end
-| _18_195 -> begin
+| _21_195 -> begin
 Util.Err ((FStar.String.strcat "Cannot reduce assertion: " (ExprTypes.show tm)))
 end)
 end
@@ -307,17 +307,17 @@ end
 | ExprTypes.BEXP (bexp) -> begin
 (
 
-let _18_200 = (interp.alloc st bexp)
-in (match (_18_200) with
+let _21_200 = (interp.alloc st bexp)
+in (match (_21_200) with
 | (l, st') -> begin
 Util.Val ((ExprTypes.LOC (l), st'))
 end))
 end
-| _18_202 -> begin
+| _21_202 -> begin
 Util.Err ((FStar.String.strcat "No rule applies: " (ExprTypes.show tm)))
 end)
 end))
-and step_lst = (fun ( _18_205  :  'Astate listconfig ) ( interp  :  'Astate interpretation ) -> (match (_18_205) with
+and step_lst = (fun ( _21_205  :  'Astate listconfig ) ( interp  :  'Astate interpretation ) -> (match (_21_205) with
 | (lst, st) -> begin
 (match (lst) with
 | [] -> begin
@@ -325,12 +325,12 @@ Util.Val (([], st))
 end
 | x::xs -> begin
 if (not ((isVal x))) then begin
-(Util.bindT (step (x, st) interp) (fun ( _18_213  :  'Astate config ) -> (match (_18_213) with
+(Util.bindT (step (x, st) interp) (fun ( _21_213  :  'Astate config ) -> (match (_21_213) with
 | (x', st') -> begin
 Util.Val (((x')::xs, st'))
 end)))
 end else begin
-(Util.bindT (step_lst (xs, st) interp) (fun ( _18_216  :  'Astate listconfig ) -> (match (_18_216) with
+(Util.bindT (step_lst (xs, st) interp) (fun ( _21_216  :  'Astate listconfig ) -> (match (_21_216) with
 | (xs', st') -> begin
 Util.Val (((x)::xs', st'))
 end)))
@@ -339,11 +339,11 @@ end)
 end))
 
 
-let rec eval_rec = (fun ( _18_221  :  'Astate config ) ( interp  :  'Astate interpretation ) -> (match (_18_221) with
+let rec eval_rec = (fun ( _21_221  :  'Astate config ) ( interp  :  'Astate interpretation ) -> (match (_21_221) with
 | (tm, st) -> begin
 (match (tm) with
 | ExprTypes.LET (x, t1, t2) -> begin
-(Util.bind (eval_rec (t1, st) interp) (fun ( _18_230  :  'Astate config ) -> (match (_18_230) with
+(Util.bind (eval_rec (t1, st) interp) (fun ( _21_230  :  'Astate config ) -> (match (_21_230) with
 | (v1, st') -> begin
 (eval_rec ((ExprTypes.substGExpr t2 x v1), st') interp)
 end)))
@@ -352,36 +352,36 @@ end
 Util.Val ((tm, st))
 end
 | ExprTypes.APPLY (t1, t2) -> begin
-(Util.bind (eval_rec (t1, st) interp) (fun ( _18_242  :  'Astate config ) -> (match (_18_242) with
+(Util.bind (eval_rec (t1, st) interp) (fun ( _21_242  :  'Astate config ) -> (match (_21_242) with
 | (v1, st') -> begin
-(Util.bind (eval_rec (t2, st') interp) (fun ( _18_245  :  'Astate config ) -> (match (_18_245) with
+(Util.bind (eval_rec (t2, st') interp) (fun ( _21_245  :  'Astate config ) -> (match (_21_245) with
 | (v2, st'') -> begin
 (match (v1) with
 | ExprTypes.LAMBDA (x, ty, t) -> begin
 (eval_rec ((ExprTypes.substGExpr t x v2), st'') interp)
 end
-| _18_252 -> begin
+| _21_252 -> begin
 Util.Err ((FStar.String.strcat "LHS is not a lambda: " (ExprTypes.show tm)))
 end)
 end)))
 end)))
 end
 | ExprTypes.SEQUENCE (t1, t2) -> begin
-(Util.bind (eval_rec (t1, st) interp) (fun ( _18_259  :  'Astate config ) -> (match (_18_259) with
+(Util.bind (eval_rec (t1, st) interp) (fun ( _21_259  :  'Astate config ) -> (match (_21_259) with
 | (v1, st') -> begin
 (eval_rec (t2, st') interp)
 end)))
 end
 | ExprTypes.ASSIGN (t1, t2) -> begin
-(Util.bind (eval_rec (t1, st) interp) (fun ( _18_266  :  'Astate config ) -> (match (_18_266) with
+(Util.bind (eval_rec (t1, st) interp) (fun ( _21_266  :  'Astate config ) -> (match (_21_266) with
 | (v1, st') -> begin
-(Util.bind (eval_rec (t2, st') interp) (fun ( _18_269  :  'Astate config ) -> (match (_18_269) with
+(Util.bind (eval_rec (t2, st') interp) (fun ( _21_269  :  'Astate config ) -> (match (_21_269) with
 | (v2, st'') -> begin
 (match ((v1, v2)) with
 | (ExprTypes.LOC (l), ExprTypes.BEXP (bexp)) -> begin
 Util.Val ((ExprTypes.UNIT, (interp.assign st' l bexp)))
 end
-| _18_276 -> begin
+| _21_276 -> begin
 Util.Err ((FStar.String.strcat "Invalid parameters: " (ExprTypes.show tm)))
 end)
 end)))
@@ -391,48 +391,48 @@ end
 (Util.bind (eval_to_bexp (tm, st) interp) (fun ( c  :  'Astate config ) -> (eval_rec c interp)))
 end
 | ExprTypes.APPEND (t1, t2) -> begin
-(Util.bind (eval_rec (t1, st) interp) (fun ( _18_293  :  'Astate config ) -> (match (_18_293) with
+(Util.bind (eval_rec (t1, st) interp) (fun ( _21_293  :  'Astate config ) -> (match (_21_293) with
 | (v1, st') -> begin
-(Util.bind (eval_rec (t2, st') interp) (fun ( _18_296  :  'Astate config ) -> (match (_18_296) with
+(Util.bind (eval_rec (t2, st') interp) (fun ( _21_296  :  'Astate config ) -> (match (_21_296) with
 | (v2, st'') -> begin
 (match ((v1, v2)) with
 | (ExprTypes.ARRAY (l1), ExprTypes.ARRAY (l2)) -> begin
 Util.Val ((ExprTypes.ARRAY ((FStar.List.append l1 l2)), st''))
 end
-| _18_303 -> begin
+| _21_303 -> begin
 Util.Err ((FStar.String.strcat "Append of non-array argument: " (ExprTypes.show tm)))
 end)
 end)))
 end)))
 end
 | ExprTypes.ROT (i, t) -> begin
-(Util.bind (eval_rec (t, st) interp) (fun ( _18_310  :  'Astate config ) -> (match (_18_310) with
+(Util.bind (eval_rec (t, st) interp) (fun ( _21_310  :  'Astate config ) -> (match (_21_310) with
 | (v, st') -> begin
 (match (v) with
 | ExprTypes.ARRAY (lst) -> begin
-if ((0 <= i) && (i < (FStar.List.length lst))) then begin
+if (((Prims.parse_int "0") <= i) && (i < (FStar.List.length lst))) then begin
 Util.Val ((ExprTypes.ARRAY ((Util.rotate lst i)), st'))
 end else begin
 Util.Err ((FStar.String.strcat "Rotation out of array bounds: " (ExprTypes.show tm)))
 end
 end
-| _18_314 -> begin
+| _21_314 -> begin
 Util.Err ((FStar.String.strcat "Rotation of non-array argument: " (ExprTypes.show tm)))
 end)
 end)))
 end
 | ExprTypes.SLICE (t, i, j) -> begin
-(Util.bind (eval_rec (t, st) interp) (fun ( _18_322  :  'Astate config ) -> (match (_18_322) with
+(Util.bind (eval_rec (t, st) interp) (fun ( _21_322  :  'Astate config ) -> (match (_21_322) with
 | (v, st') -> begin
 (match (v) with
 | ExprTypes.ARRAY (lst) -> begin
-if (((0 <= i) && (i <= j)) && (j < (FStar.List.length lst))) then begin
+if ((((Prims.parse_int "0") <= i) && (i <= j)) && (j < (FStar.List.length lst))) then begin
 Util.Val ((ExprTypes.ARRAY ((Util.slice lst i j)), st'))
 end else begin
 Util.Err ((FStar.String.strcat "Invalid slice bounds: " (ExprTypes.show tm)))
 end
 end
-| _18_326 -> begin
+| _21_326 -> begin
 Util.Err ((FStar.String.strcat "Slice of non-array argument: " (ExprTypes.show tm)))
 end)
 end)))
@@ -440,35 +440,35 @@ end
 | ExprTypes.ARRAY (tlst) -> begin
 (
 
-let f = (fun ( _18_332  :  (ExprTypes.l__GExpr Prims.list * 'Astate) ) ( t  :  ExprTypes.l__GExpr ) -> (match (_18_332) with
+let f = (fun ( _21_332  :  (ExprTypes.l__GExpr Prims.list * 'Astate) ) ( t  :  ExprTypes.l__GExpr ) -> (match (_21_332) with
 | (acc, st) -> begin
-(Util.bind (eval_rec (t, st) interp) (fun ( _18_336  :  'Astate config ) -> (match (_18_336) with
+(Util.bind (eval_rec (t, st) interp) (fun ( _21_336  :  'Astate config ) -> (match (_21_336) with
 | (v, st') -> begin
 (match (v) with
 | ExprTypes.LOC (l) -> begin
 Util.Val (((v)::acc, st'))
 end
-| _18_340 -> begin
+| _21_340 -> begin
 Util.Err ((FStar.String.strcat "Array argument not boolean: " (ExprTypes.show t)))
 end)
 end)))
 end))
-in (Util.bind (Util.foldM f ([], st) tlst) (fun ( _18_343  :  (ExprTypes.l__GExpr Prims.list * 'Astate) ) -> (match (_18_343) with
+in (Util.bind (Util.foldM f ([], st) tlst) (fun ( _21_343  :  (ExprTypes.l__GExpr Prims.list * 'Astate) ) -> (match (_21_343) with
 | (llst, st') -> begin
 Util.Val ((ExprTypes.ARRAY ((FStar.List.rev llst)), st'))
 end))))
 end
 | ExprTypes.GET_ARRAY (t, i) -> begin
-(Util.bind (eval_rec (t, st) interp) (fun ( _18_350  :  'Astate config ) -> (match (_18_350) with
+(Util.bind (eval_rec (t, st) interp) (fun ( _21_350  :  'Astate config ) -> (match (_21_350) with
 | (v, st') -> begin
 (match (v) with
 | ExprTypes.ARRAY (lst) -> begin
-if ((0 <= i) && (i < (FStar.List.length lst))) then begin
+if (((Prims.parse_int "0") <= i) && (i < (FStar.List.length lst))) then begin
 (match ((FStar.List.total_nth lst i)) with
 | Some (ExprTypes.LOC (l)) -> begin
 Util.Val ((ExprTypes.LOC (l), st'))
 end
-| Some (_18_357) -> begin
+| Some (_21_357) -> begin
 Util.Err ("Impossible")
 end
 | None -> begin
@@ -478,7 +478,7 @@ end else begin
 Util.Err ((FStar.String.strcat "Array out of bounds: " (ExprTypes.show tm)))
 end
 end
-| _18_361 -> begin
+| _21_361 -> begin
 Util.Err ((FStar.String.strcat "Invalid parameters: " (ExprTypes.show tm)))
 end)
 end)))
@@ -487,13 +487,13 @@ end
 Util.Val ((tm, st))
 end
 | ExprTypes.ASSERT (t) -> begin
-(Util.bind (eval_rec (t, st) interp) (fun ( _18_368  :  'Astate config ) -> (match (_18_368) with
+(Util.bind (eval_rec (t, st) interp) (fun ( _21_368  :  'Astate config ) -> (match (_21_368) with
 | (v, st') -> begin
 (match (v) with
 | ExprTypes.LOC (l) -> begin
 Util.Val ((ExprTypes.UNIT, st'))
 end
-| _18_372 -> begin
+| _21_372 -> begin
 Util.Err ((FStar.String.strcat "Assert of non-boolean argument: " (ExprTypes.show tm)))
 end)
 end)))
@@ -501,44 +501,44 @@ end
 | ExprTypes.BEXP (bexp) -> begin
 (
 
-let _18_377 = (interp.alloc st bexp)
-in (match (_18_377) with
+let _21_377 = (interp.alloc st bexp)
+in (match (_21_377) with
 | (l, st') -> begin
 Util.Val ((ExprTypes.LOC (l), st'))
 end))
 end
-| _18_379 -> begin
+| _21_379 -> begin
 Util.Err ((FStar.String.strcat "Unimplemented case: " (ExprTypes.show tm)))
 end)
 end))
-and eval_to_bexp = (fun ( _18_382  :  'Astate config ) ( interp  :  'Astate interpretation ) -> (match (_18_382) with
+and eval_to_bexp = (fun ( _21_382  :  'Astate config ) ( interp  :  'Astate interpretation ) -> (match (_21_382) with
 | (tm, st) -> begin
 (match (tm) with
 | ExprTypes.XOR (x, y) -> begin
-(Util.bind (eval_to_bexp (x, st) interp) (fun ( _18_390  :  'Astate config ) -> (match (_18_390) with
+(Util.bind (eval_to_bexp (x, st) interp) (fun ( _21_390  :  'Astate config ) -> (match (_21_390) with
 | (x', st') -> begin
-(Util.bind (eval_to_bexp (y, st') interp) (fun ( _18_393  :  'Astate config ) -> (match (_18_393) with
+(Util.bind (eval_to_bexp (y, st') interp) (fun ( _21_393  :  'Astate config ) -> (match (_21_393) with
 | (y', st'') -> begin
 (match ((x', y')) with
 | (ExprTypes.BEXP (b), ExprTypes.BEXP (b')) -> begin
 Util.Val ((ExprTypes.BEXP (BoolExp.BXor ((b, b'))), st''))
 end
-| _18_400 -> begin
+| _21_400 -> begin
 Util.Err ((FStar.String.strcat "Could not reduce parameters to booleans: " (ExprTypes.show tm)))
 end)
 end)))
 end)))
 end
 | ExprTypes.AND (x, y) -> begin
-(Util.bind (eval_to_bexp (x, st) interp) (fun ( _18_407  :  'Astate config ) -> (match (_18_407) with
+(Util.bind (eval_to_bexp (x, st) interp) (fun ( _21_407  :  'Astate config ) -> (match (_21_407) with
 | (x', st') -> begin
-(Util.bind (eval_to_bexp (y, st') interp) (fun ( _18_410  :  'Astate config ) -> (match (_18_410) with
+(Util.bind (eval_to_bexp (y, st') interp) (fun ( _21_410  :  'Astate config ) -> (match (_21_410) with
 | (y', st'') -> begin
 (match ((x', y')) with
 | (ExprTypes.BEXP (b), ExprTypes.BEXP (b')) -> begin
 Util.Val ((ExprTypes.BEXP (BoolExp.BAnd ((b, b'))), st''))
 end
-| _18_417 -> begin
+| _21_417 -> begin
 Util.Err ((FStar.String.strcat "Could not reduce parameters to booleans: " (ExprTypes.show tm)))
 end)
 end)))
@@ -551,14 +551,14 @@ end else begin
 Util.Val ((ExprTypes.BEXP (BoolExp.BFalse), st))
 end
 end
-| _18_421 -> begin
-(Util.bind (eval_rec (tm, st) interp) (fun ( _18_424  :  'Astate config ) -> (match (_18_424) with
+| _21_421 -> begin
+(Util.bind (eval_rec (tm, st) interp) (fun ( _21_424  :  'Astate config ) -> (match (_21_424) with
 | (v, st') -> begin
 (match (v) with
 | ExprTypes.LOC (l) -> begin
 Util.Val ((ExprTypes.BEXP (BoolExp.BVar (l)), st'))
 end
-| _18_428 -> begin
+| _21_428 -> begin
 Util.Err ((FStar.String.strcat "Could not reduce expression to boolean: " (ExprTypes.show tm)))
 end)
 end)))
@@ -570,22 +570,22 @@ type boolState =
 (Prims.int * (Prims.int, Prims.bool) Total.map)
 
 
-let boolInit : (Prims.int * (Prims.int  ->  Prims.bool)) = (0, (Total.const false))
+let boolInit : (Prims.int * (Prims.int  ->  Prims.bool)) = ((Prims.parse_int "0"), (Total.const_map false))
 
 
-let boolAlloc : boolState  ->  BoolExp.l__BoolExp  ->  (Prims.int * boolState) = (fun ( _18_431  :  boolState ) ( bexp  :  BoolExp.l__BoolExp ) -> (match (_18_431) with
+let boolAlloc : boolState  ->  BoolExp.l__BoolExp  ->  (Prims.int * boolState) = (fun ( _21_431  :  boolState ) ( bexp  :  BoolExp.l__BoolExp ) -> (match (_21_431) with
 | (top, st) -> begin
-(top, ((top + 1), (Total.update st top (BoolExp.evalBexp bexp st))))
+(top, ((top + (Prims.parse_int "1")), (Total.update st top (BoolExp.evalBexp bexp st))))
 end))
 
 
-let boolAssign : boolState  ->  Prims.int  ->  BoolExp.l__BoolExp  ->  boolState = (fun ( _18_435  :  boolState ) ( l  :  Prims.int ) ( bexp  :  BoolExp.l__BoolExp ) -> (match (_18_435) with
+let boolAssign : boolState  ->  Prims.int  ->  BoolExp.l__BoolExp  ->  boolState = (fun ( _21_435  :  boolState ) ( l  :  Prims.int ) ( bexp  :  BoolExp.l__BoolExp ) -> (match (_21_435) with
 | (top, st) -> begin
 (top, (Total.update st l (BoolExp.evalBexp bexp st)))
 end))
 
 
-let boolEval : boolState  ->  Total.state  ->  Prims.int  ->  Prims.bool = (fun ( _18_440  :  boolState ) ( ivals  :  Total.state ) ( i  :  Prims.int ) -> (match (_18_440) with
+let boolEval : boolState  ->  Total.state  ->  Prims.int  ->  Prims.bool = (fun ( _21_440  :  boolState ) ( ivals  :  Total.state ) ( i  :  Prims.int ) -> (match (_21_440) with
 | (top, st) -> begin
 (Total.lookup st i)
 end))
@@ -613,7 +613,7 @@ end
 end))
 
 
-let rec evalBool : (ExprTypes.l__GExpr * (Prims.int * (Prims.int  ->  Prims.bool)))  ->  Prims.string Prims.list = (fun ( _18_468  :  (ExprTypes.l__GExpr * (Prims.int * (Prims.int  ->  Prims.bool))) ) -> (match (_18_468) with
+let rec evalBool : (ExprTypes.l__GExpr * (Prims.int * (Prims.int  ->  Prims.bool)))  ->  Prims.string Prims.list = (fun ( _21_468  :  (ExprTypes.l__GExpr * (Prims.int * (Prims.int  ->  Prims.bool))) ) -> (match (_21_468) with
 | (gexp, st) -> begin
 if (isVal gexp) then begin
 (ExprTypes.prettyPrint (substVal gexp st))
@@ -636,22 +636,22 @@ type l__BExpState =
 (Prims.int * (Prims.int, BoolExp.l__BoolExp) Total.map)
 
 
-let bexpInit : (Prims.int * (Prims.int  ->  BoolExp.l__BoolExp)) = (0, (Total.const BoolExp.BFalse))
+let bexpInit : (Prims.int * (Prims.int  ->  BoolExp.l__BoolExp)) = ((Prims.parse_int "0"), (Total.const_map BoolExp.BFalse))
 
 
-let bexpAlloc : l__BExpState  ->  BoolExp.l__BoolExp  ->  (Prims.int * l__BExpState) = (fun ( _18_476  :  l__BExpState ) ( bexp  :  BoolExp.l__BoolExp ) -> (match (_18_476) with
+let bexpAlloc : l__BExpState  ->  BoolExp.l__BoolExp  ->  (Prims.int * l__BExpState) = (fun ( _21_476  :  l__BExpState ) ( bexp  :  BoolExp.l__BoolExp ) -> (match (_21_476) with
 | (top, st) -> begin
-(top, ((top + 1), (Total.update st top (BoolExp.substBexp bexp st))))
+(top, ((top + (Prims.parse_int "1")), (Total.update st top (BoolExp.substBexp bexp st))))
 end))
 
 
-let bexpAssign : l__BExpState  ->  Prims.int  ->  BoolExp.l__BoolExp  ->  l__BExpState = (fun ( _18_480  :  l__BExpState ) ( l  :  Prims.int ) ( bexp  :  BoolExp.l__BoolExp ) -> (match (_18_480) with
+let bexpAssign : l__BExpState  ->  Prims.int  ->  BoolExp.l__BoolExp  ->  l__BExpState = (fun ( _21_480  :  l__BExpState ) ( l  :  Prims.int ) ( bexp  :  BoolExp.l__BoolExp ) -> (match (_21_480) with
 | (top, st) -> begin
 (top, (Total.update st l (BoolExp.substBexp bexp st)))
 end))
 
 
-let bexpEval : l__BExpState  ->  Total.state  ->  Prims.int  ->  Prims.bool = (fun ( _18_485  :  l__BExpState ) ( ivals  :  Total.state ) ( i  :  Prims.int ) -> (match (_18_485) with
+let bexpEval : l__BExpState  ->  Total.state  ->  Prims.int  ->  Prims.bool = (fun ( _21_485  :  l__BExpState ) ( ivals  :  Total.state ) ( i  :  Prims.int ) -> (match (_21_485) with
 | (top, st) -> begin
 (BoolExp.evalBexp (Total.lookup st i) ivals)
 end))
@@ -696,32 +696,32 @@ end))
 let simps : BoolExp.l__BoolExp  ->  BoolExp.l__BoolExp = (fun ( bexp  :  BoolExp.l__BoolExp ) -> (BoolExp.simplify (BoolExp.distributeAnds bexp)))
 
 
-let rec allocN : (ExprTypes.l__GExpr Prims.list * l__BExpState)  ->  Prims.int  ->  (ExprTypes.l__GExpr Prims.list * l__BExpState) = (fun ( _18_494  :  (ExprTypes.l__GExpr Prims.list * l__BExpState) ) ( i  :  Prims.int ) -> (match (_18_494) with
+let rec allocN : (ExprTypes.l__GExpr Prims.list * l__BExpState)  ->  Prims.int  ->  (ExprTypes.l__GExpr Prims.list * l__BExpState) = (fun ( _21_494  :  (ExprTypes.l__GExpr Prims.list * l__BExpState) ) ( i  :  Prims.int ) -> (match (_21_494) with
 | (locs, (top, st)) -> begin
-if (i <= 0) then begin
+if (i <= (Prims.parse_int "0")) then begin
 ((FStar.List.rev locs), (top, st))
 end else begin
-(allocN ((ExprTypes.LOC (top))::locs, ((top + 1), (Total.update st top (BoolExp.BVar (top))))) (i - 1))
+(allocN ((ExprTypes.LOC (top))::locs, ((top + (Prims.parse_int "1")), (Total.update st top (BoolExp.BVar (top))))) (i - (Prims.parse_int "1")))
 end
 end))
 
 
-let allocTy : ExprTypes.l__GType  ->  l__BExpState  ->  (ExprTypes.l__GExpr * l__BExpState) Util.result = (fun ( ty  :  ExprTypes.l__GType ) ( _18_499  :  l__BExpState ) -> (match (_18_499) with
+let allocTy : ExprTypes.l__GType  ->  l__BExpState  ->  (ExprTypes.l__GExpr * l__BExpState) Util.result = (fun ( ty  :  ExprTypes.l__GType ) ( _21_499  :  l__BExpState ) -> (match (_21_499) with
 | (top, st) -> begin
 (match (ty) with
 | ExprTypes.GBool -> begin
-Util.Val ((ExprTypes.LOC (top), ((top + 1), (Total.update st top (BoolExp.BVar (top))))))
+Util.Val ((ExprTypes.LOC (top), ((top + (Prims.parse_int "1")), (Total.update st top (BoolExp.BVar (top))))))
 end
 | ExprTypes.GArray (n) -> begin
 (
 
-let _18_505 = (allocN ([], (top, st)) n)
-in (match (_18_505) with
+let _21_505 = (allocN ([], (top, st)) n)
+in (match (_21_505) with
 | (locs, st') -> begin
 Util.Val ((ExprTypes.ARRAY (locs), st'))
 end))
 end
-| _18_507 -> begin
+| _21_507 -> begin
 Util.Err ("Invalid parameter type for circuit generation")
 end)
 end))
@@ -736,43 +736,43 @@ end
 end))
 
 
-let foldPebble : (AncillaHeap.l__AncHeap * Prims.int Prims.list * Prims.int Prims.list * Circuit.l__Gate Prims.list)  ->  BoolExp.l__BoolExp  ->  (AncillaHeap.l__AncHeap * Prims.int Prims.list * Prims.int Prims.list * Circuit.l__Gate Prims.list) = (fun ( _18_522  :  (AncillaHeap.l__AncHeap * Prims.int Prims.list * Prims.int Prims.list * Circuit.l__Gate Prims.list) ) ( bexp  :  BoolExp.l__BoolExp ) -> (match (_18_522) with
+let foldPebble : (AncillaHeap.l__AncHeap * Prims.int Prims.list * Prims.int Prims.list * Circuit.l__Gate Prims.list)  ->  BoolExp.l__BoolExp  ->  (AncillaHeap.l__AncHeap * Prims.int Prims.list * Prims.int Prims.list * Circuit.l__Gate Prims.list) = (fun ( _21_522  :  (AncillaHeap.l__AncHeap * Prims.int Prims.list * Prims.int Prims.list * Circuit.l__Gate Prims.list) ) ( bexp  :  BoolExp.l__BoolExp ) -> (match (_21_522) with
 | (ah, outs, anc, circ) -> begin
 (
 
-let _18_528 = (BoolExp.compileBexpPebbled_oop ah (simps bexp))
-in (match (_18_528) with
+let _21_528 = (BoolExp.compileBexpPebbled_oop ah (simps bexp))
+in (match (_21_528) with
 | (ah', res, anc', circ') -> begin
 (ah', (res)::outs, (FStar.List.append anc' anc), (FStar.List.append circ circ'))
 end))
 end))
 
 
-let foldClean : (AncillaHeap.l__AncHeap * Prims.int Prims.list * Prims.int Prims.list * Circuit.l__Gate Prims.list)  ->  BoolExp.l__BoolExp  ->  (AncillaHeap.l__AncHeap * Prims.int Prims.list * Prims.int Prims.list * Circuit.l__Gate Prims.list) = (fun ( _18_533  :  (AncillaHeap.l__AncHeap * Prims.int Prims.list * Prims.int Prims.list * Circuit.l__Gate Prims.list) ) ( bexp  :  BoolExp.l__BoolExp ) -> (match (_18_533) with
+let foldClean : (AncillaHeap.l__AncHeap * Prims.int Prims.list * Prims.int Prims.list * Circuit.l__Gate Prims.list)  ->  BoolExp.l__BoolExp  ->  (AncillaHeap.l__AncHeap * Prims.int Prims.list * Prims.int Prims.list * Circuit.l__Gate Prims.list) = (fun ( _21_533  :  (AncillaHeap.l__AncHeap * Prims.int Prims.list * Prims.int Prims.list * Circuit.l__Gate Prims.list) ) ( bexp  :  BoolExp.l__BoolExp ) -> (match (_21_533) with
 | (ah, outs, anc, circ) -> begin
 (
 
-let _18_539 = (BoolExp.compileBexpClean_oop ah (simps bexp))
-in (match (_18_539) with
+let _21_539 = (BoolExp.compileBexpClean_oop ah (simps bexp))
+in (match (_21_539) with
 | (ah', res, anc', circ') -> begin
 (ah', (res)::outs, (FStar.List.append anc' anc), (FStar.List.append circ circ'))
 end))
 end))
 
 
-let foldBennett : (AncillaHeap.l__AncHeap * Prims.int Prims.list * Prims.int Prims.list * Circuit.l__Gate Prims.list * Circuit.l__Gate Prims.list)  ->  BoolExp.l__BoolExp  ->  (AncillaHeap.l__AncHeap * Prims.int Prims.list * Prims.int Prims.list * Circuit.l__Gate Prims.list * Circuit.l__Gate Prims.list) = (fun ( _18_545  :  (AncillaHeap.l__AncHeap * Prims.int Prims.list * Prims.int Prims.list * Circuit.l__Gate Prims.list * Circuit.l__Gate Prims.list) ) ( bexp  :  BoolExp.l__BoolExp ) -> (match (_18_545) with
+let foldBennett : (AncillaHeap.l__AncHeap * Prims.int Prims.list * Prims.int Prims.list * Circuit.l__Gate Prims.list * Circuit.l__Gate Prims.list)  ->  BoolExp.l__BoolExp  ->  (AncillaHeap.l__AncHeap * Prims.int Prims.list * Prims.int Prims.list * Circuit.l__Gate Prims.list * Circuit.l__Gate Prims.list) = (fun ( _21_545  :  (AncillaHeap.l__AncHeap * Prims.int Prims.list * Prims.int Prims.list * Circuit.l__Gate Prims.list * Circuit.l__Gate Prims.list) ) ( bexp  :  BoolExp.l__BoolExp ) -> (match (_21_545) with
 | (ah, outs, anc, circ, ucirc) -> begin
 (
 
-let _18_551 = (BoolExp.compileBexp_oop ah (simps bexp))
-in (match (_18_551) with
+let _21_551 = (BoolExp.compileBexp_oop ah (simps bexp))
+in (match (_21_551) with
 | (ah', res, anc', circ') -> begin
 (ah', (res)::outs, (FStar.List.append anc' anc), (FStar.List.append circ circ'), (FStar.List.append (FStar.List.rev (Circuit.uncompute circ' res)) ucirc))
 end))
 end))
 
 
-let rec compile : l__BExpState config  ->  l__CleanupStrategy  ->  (Prims.int Prims.list * Circuit.l__Gate Prims.list) Util.result = (fun ( _18_554  :  l__BExpState config ) ( strategy  :  l__CleanupStrategy ) -> (match (_18_554) with
+let rec compile : l__BExpState config  ->  l__CleanupStrategy  ->  (Prims.int Prims.list * Circuit.l__Gate Prims.list) Util.result = (fun ( _21_554  :  l__BExpState config ) ( strategy  :  l__CleanupStrategy ) -> (match (_21_554) with
 | (gexp, st) -> begin
 if (isVal gexp) then begin
 (match (gexp) with
@@ -797,17 +797,17 @@ in (
 let max = (BoolExp.varMax bexp)
 in (
 
-let _18_579 = (match (strategy) with
+let _21_579 = (match (strategy) with
 | Pebbled -> begin
-(BoolExp.compileBexpPebbled_oop (AncillaHeap.above (max + 1)) (simps bexp))
+(BoolExp.compileBexpPebbled_oop (AncillaHeap.above (max + (Prims.parse_int "1"))) (simps bexp))
 end
 | Boundaries -> begin
-(BoolExp.compileBexpClean_oop (AncillaHeap.above (max + 1)) (simps bexp))
+(BoolExp.compileBexpClean_oop (AncillaHeap.above (max + (Prims.parse_int "1"))) (simps bexp))
 end
 | Bennett -> begin
-(BoolExp.compileBexpClean_oop (AncillaHeap.above (max + 1)) (simps bexp))
+(BoolExp.compileBexpClean_oop (AncillaHeap.above (max + (Prims.parse_int "1"))) (simps bexp))
 end)
-in (match (_18_579) with
+in (match (_21_579) with
 | (ah, res, anc, circ) -> begin
 Util.Val (((res)::[], circ))
 end))))
@@ -821,12 +821,12 @@ in (
 let max = (BoolExp.listMax (FStar.List.mapT BoolExp.varMax blst))
 in (
 
-let _18_607 = (match (strategy) with
+let _21_607 = (match (strategy) with
 | Pebbled -> begin
 (
 
-let _18_589 = (FStar.List.fold_leftT foldPebble ((AncillaHeap.above (max + 1)), [], [], []) blst)
-in (match (_18_589) with
+let _21_589 = (FStar.List.fold_leftT foldPebble ((AncillaHeap.above (max + (Prims.parse_int "1"))), [], [], []) blst)
+in (match (_21_589) with
 | (ah, outs, anc, circ) -> begin
 (ah, (FStar.List.rev outs), (FStar.List.rev anc), circ)
 end))
@@ -834,8 +834,8 @@ end
 | Boundaries -> begin
 (
 
-let _18_595 = (FStar.List.fold_leftT foldClean ((AncillaHeap.above (max + 1)), [], [], []) blst)
-in (match (_18_595) with
+let _21_595 = (FStar.List.fold_leftT foldClean ((AncillaHeap.above (max + (Prims.parse_int "1"))), [], [], []) blst)
+in (match (_21_595) with
 | (ah, outs, anc, circ) -> begin
 (ah, (FStar.List.rev outs), (FStar.List.rev anc), circ)
 end))
@@ -843,13 +843,13 @@ end
 | Bennett -> begin
 (
 
-let _18_602 = (FStar.List.fold_leftT foldBennett ((AncillaHeap.above (max + 1)), [], [], [], []) blst)
-in (match (_18_602) with
+let _21_602 = (FStar.List.fold_leftT foldBennett ((AncillaHeap.above (max + (Prims.parse_int "1"))), [], [], [], []) blst)
+in (match (_21_602) with
 | (ah, outs, anc, circ, ucirc) -> begin
 (ah, (FStar.List.rev outs), (FStar.List.rev anc), (FStar.List.append circ ucirc))
 end))
 end)
-in (match (_18_607) with
+in (match (_21_607) with
 | (ah, outs, anc, circ) -> begin
 Util.Val ((outs, circ))
 end))))
@@ -873,17 +873,17 @@ type circState =
 let is_MkcircState : circState  ->  Prims.bool = (Prims.checked_cast(fun ( _  :  circState ) -> (FStar.All.failwith "Not yet implemented:is_MkcircState")))
 
 
-let circInit : circState = {top = 0; ah = AncillaHeap.emptyHeap; gates = []; subs = (Total.const 0)}
+let circInit : circState = {top = (Prims.parse_int "0"); ah = AncillaHeap.emptyHeap; gates = []; subs = (Total.const_map (Prims.parse_int "0"))}
 
 
 let circAlloc : circState  ->  BoolExp.l__BoolExp  ->  (Prims.int * circState) = (fun ( cs  :  circState ) ( bexp  :  BoolExp.l__BoolExp ) -> (
 
-let _18_623 = (BoolExp.compileBexp_oop cs.ah (BoolExp.substVar bexp cs.subs))
-in (match (_18_623) with
+let _21_623 = (BoolExp.compileBexp_oop cs.ah (BoolExp.substVar bexp cs.subs))
+in (match (_21_623) with
 | (ah', res, ancs, circ') -> begin
 (
 
-let top' = (cs.top + 1)
+let top' = (cs.top + (Prims.parse_int "1"))
 in (
 
 let gates' = (FStar.List.append cs.gates circ')
@@ -902,14 +902,14 @@ in (
 let bexp' = (BoolExp.substVar bexp cs.subs)
 in (
 
-let _18_639 = (match ((BoolExp.factorAs bexp' l')) with
+let _21_639 = (match ((BoolExp.factorAs bexp' l')) with
 | None -> begin
 (BoolExp.compileBexp_oop cs.ah bexp')
 end
 | Some (bexp'') -> begin
 (BoolExp.compileBexp cs.ah l' bexp'')
 end)
-in (match (_18_639) with
+in (match (_21_639) with
 | (ah', res, ancs, circ') -> begin
 {top = cs.top; ah = ah'; gates = (FStar.List.append cs.gates circ'); subs = (Total.update cs.subs l res)}
 end)))))
@@ -921,20 +921,20 @@ let circEval : circState  ->  Total.state  ->  Prims.int  ->  Prims.bool = (fun 
 let circInterp : circState interpretation = {alloc = circAlloc; assign = circAssign; eval = circEval}
 
 
-let rec allocNcirc : (ExprTypes.l__GExpr Prims.list * circState)  ->  Prims.int  ->  (ExprTypes.l__GExpr Prims.list * circState) = (fun ( _18_646  :  (ExprTypes.l__GExpr Prims.list * circState) ) ( i  :  Prims.int ) -> (match (_18_646) with
+let rec allocNcirc : (ExprTypes.l__GExpr Prims.list * circState)  ->  Prims.int  ->  (ExprTypes.l__GExpr Prims.list * circState) = (fun ( _21_646  :  (ExprTypes.l__GExpr Prims.list * circState) ) ( i  :  Prims.int ) -> (match (_21_646) with
 | (locs, cs) -> begin
-if (i <= 0) then begin
+if (i <= (Prims.parse_int "0")) then begin
 ((FStar.List.rev locs), cs)
 end else begin
 (
 
-let _18_650 = (AncillaHeap.popMin cs.ah)
-in (match (_18_650) with
+let _21_650 = (AncillaHeap.popMin cs.ah)
+in (match (_21_650) with
 | (ah', res) -> begin
 (
 
-let cs' = {top = (cs.top + 1); ah = ah'; gates = cs.gates; subs = (Total.update cs.subs cs.top res)}
-in (allocNcirc ((ExprTypes.LOC (cs.top))::locs, cs') (i - 1)))
+let cs' = {top = (cs.top + (Prims.parse_int "1")); ah = ah'; gates = cs.gates; subs = (Total.update cs.subs cs.top res)}
+in (allocNcirc ((ExprTypes.LOC (cs.top))::locs, cs') (i - (Prims.parse_int "1"))))
 end))
 end
 end))
@@ -944,25 +944,25 @@ let allocTycirc : ExprTypes.l__GType  ->  circState  ->  (ExprTypes.l__GExpr * c
 | ExprTypes.GBool -> begin
 (
 
-let _18_657 = (AncillaHeap.popMin cs.ah)
-in (match (_18_657) with
+let _21_657 = (AncillaHeap.popMin cs.ah)
+in (match (_21_657) with
 | (ah', res) -> begin
 (
 
-let cs' = {top = (cs.top + 1); ah = ah'; gates = cs.gates; subs = (Total.update cs.subs cs.top res)}
+let cs' = {top = (cs.top + (Prims.parse_int "1")); ah = ah'; gates = cs.gates; subs = (Total.update cs.subs cs.top res)}
 in Util.Val ((ExprTypes.LOC (cs.top), cs')))
 end))
 end
 | ExprTypes.GArray (n) -> begin
 (
 
-let _18_663 = (allocNcirc ([], cs) n)
-in (match (_18_663) with
+let _21_663 = (allocNcirc ([], cs) n)
+in (match (_21_663) with
 | (locs, st') -> begin
 Util.Val ((ExprTypes.ARRAY (locs), st'))
 end))
 end
-| _18_665 -> begin
+| _21_665 -> begin
 Util.Err ("Invalid parameter type for circuit generation")
 end))
 
@@ -976,7 +976,7 @@ end
 end))
 
 
-let rec compileCirc : circState config  ->  (Prims.int Prims.list * Circuit.l__Gate Prims.list) Util.result = (fun ( _18_678  :  circState config ) -> (match (_18_678) with
+let rec compileCirc : circState config  ->  (Prims.int Prims.list * Circuit.l__Gate Prims.list) Util.result = (fun ( _21_678  :  circState config ) -> (match (_21_678) with
 | (gexp, cs) -> begin
 if (isVal gexp) then begin
 (match (gexp) with
