Makefile
@@ -1,17 +1,27 @@
 FSTAR_HOME = /home/meamy/Programming/FStar
 
 FSTAR = $(FSTAR_HOME)/bin/fstar.exe
+FSHARP = fsharpc
 
-FILES = Util.fst Maps.fst PairHeap.fst AncillaHeap.fst Circuit.fst BoolExp.fst ExprTypes.fst Interpreter.fst
+FILES = Util.fst Total.fst Par.fst PairHeap.fst AncillaHeap.fst Circuit.fst BoolExp.fst ExprTypes.fst Interpreter.fst
 STDLIB = FStar.FunctionalExtensionality.fst FStar.Set.fst FStar.Heap.fst FStar.ST.fst FStar.All.fst FStar.List.fst FStar.String.fsti
 EX = FStar.Map.fst FStar.IO.fsti FStar.ListProperties.fst
 
-SRC = $(addprefix src/, $(FILES))
-LIB = $(addprefix $(FSTAR_HOME)/lib/, $(STDLIB) $(EX))
+FSFILES =
 
-verify: $(SRC)
-	$(FSTAR) --z3timeout 60 --explicit_deps $(LIB) $^
+FSTSRC = $(addprefix src/, $(FILES))
+FSSRC  = $(addprefix src/fs/, $(STDLIB:.fst=.fs) $(EX:.fst=.fs)  $(FSFILES) $(FILES:.fst=.fs))
+LIB 	 = $(addprefix $(FSTAR_HOME)/lib/, $(STDLIB) $(EX))
 
-fs: $(SRC)
-	$(FSTAR) --admit_smt_queries true --codegen FSharp --use_native_int --explicit_deps $(LIB) $^
-	mv *.fs src/
+DLLS = $(FSTAR_HOME)/lib/fs/fstarlib.dll $(FSTAR_HOME)/bin/FSharp.PowerPack.dll $(FSTAR_HOME)/bin/FSharp.PowerPack.Compatibility.dll
+FSOPS = $(addprefix -r , $(DLLS))
+
+verify: $(FSTSRC)
+	$(FSTAR) --z3timeout 60 $^
+
+fs: $(FSTSRC)
+	$(FSTAR) --admit_smt_queries true --codegen FSharp $^
+	mv *.fs src/fs/
+
+all: $(FSSRC)
+	$(FSHARP) --mlcompatibility $(FSOPS) -o rever.exe $(FSSRC)
